Use κ for context lifetimes

nola/examples/rust_halt/base.v
@@ -168,29 +168,29 @@ Definition rust_halt_wsat
 (** ** Lifetime inclusion *)
 
 (** [LftIncl]: Type class for lifetime inclusion *)
-Class LftIncl (α β : lft) : Prop :=
-  lft_incl' : α ⊑ β.
+Class LftIncl (κ α : lft) : Prop :=
+  lft_incl' : κ ⊑ α.
 Hint Mode LftIncl ! ! : typeclass_instances.
 
 (** Trivial matches *)
-#[export] Instance lft_incl'_top {α} : LftIncl α ⊤ | 2.
+#[export] Instance lft_incl'_top {κ} : LftIncl κ ⊤ | 2.
 Proof. exact lft_incl_top. Qed.
-#[export] Instance lft_incl'_refl {α} : LftIncl α α | 2.
+#[export] Instance lft_incl'_refl {κ} : LftIncl κ κ | 2.
 Proof. exact: lft_incl_refl. Qed.
 (** Decompose the right-hand side *)
-#[export] Instance lft_incl'_meet_intro `{!LftIncl α β, !LftIncl α β'} :
-  LftIncl α (β ⊓ β') | 5.
+#[export] Instance lft_incl'_meet_intro `{!LftIncl κ α, !LftIncl κ β} :
+  LftIncl κ (α ⊓ β) | 5.
 Proof. exact: lft_incl_meet_intro. Qed.
 (** Decompose the left-hand side *)
-#[export] Instance lft_incl'_meet_by_l `{!LftIncl α β} {α'} :
-  LftIncl (α ⊓ α') β | 30.
+#[export] Instance lft_incl'_meet_by_l `{!LftIncl κ α} {κ'} :
+  LftIncl (κ ⊓ κ') α | 30.
 Proof. unfold LftIncl. etrans; [exact lft_incl_meet_l|done]. Qed.
-#[export] Instance lft_incl'_meet_by_r `{!LftIncl α' β} {α} :
-  LftIncl (α ⊓ α') β | 30.
+#[export] Instance lft_incl'_meet_by_r `{!LftIncl κ' α} {κ} :
+  LftIncl (κ ⊓ κ') α | 30.
 Proof. unfold LftIncl. etrans; [exact lft_incl_meet_r|done]. Qed.
 
-Lemma lft_incl'_live_acc `{!lftG Σ} `(!LftIncl α β) {q} :
-  q.[α] ⊢ ∃ r, r.[β] ∗ (r.[β] -∗ q.[α]).
+Lemma lft_incl'_live_acc `{!lftG Σ} `(!LftIncl κ α) {q} :
+  q.[κ] ⊢ ∃ r, r.[α] ∗ (r.[α] -∗ q.[κ]).
 Proof. by apply lft_incl_live_acc. Qed.
 
 (** ** Shared borrows *)
