nola/examples/rust_halt/ptr.v
@@ -44,37 +44,37 @@ Section read_write.
     !Jsem JUDG (iProp Σ)}.
 
   (** [Read]: Read from a pointer type *)
-  Class Read {X Y X'} (α : lft) (T : ty CON Σ X) (U : ty CON Σ Y)
+  Class Read {X Y X'} (κ : lft) (T : ty CON Σ X) (U : ty CON Σ Y)
     (T' : ty CON Σ X') (get : X → Y) (set : X → X') : Prop := READ {
     read {q t d xπ v} :
-      q.[α] -∗ na_own t ⊤ -∗ ⟦ T.1 t d xπ [v] ⟧ᶜ =[rust_halt_wsat]{⊤}=∗
+      q.[κ] -∗ na_own t ⊤ -∗ ⟦ T.1 t d xπ [v] ⟧ᶜ =[rust_halt_wsat]{⊤}=∗
         ∃ l wl du r, ⌜v = # l⌝ ∗ l ↦∗{r} wl ∗ ⟦ U.1 t du (get ∘ xπ) wl ⟧ᶜ ∗
           (l ↦∗{r} wl =[rust_halt_wsat]{⊤}=∗ ∃ d',
-            q.[α] ∗ na_own t ⊤ ∗ ⟦ T'.1 t d' (set ∘ xπ) [v] ⟧ᶜ);
+            q.[κ] ∗ na_own t ⊤ ∗ ⟦ T'.1 t d' (set ∘ xπ) [v] ⟧ᶜ);
   }.
 
   (** [Write]: Write to a pointer type *)
-  Class Write {X Y Y' X'} (α : lft) (T : ty CON Σ X) (U : ty CON Σ Y)
+  Class Write {X Y Y' X'} (κ : lft) (T : ty CON Σ X) (U : ty CON Σ Y)
     (U' : ty CON Σ Y') (T' : ty CON Σ X') (get : X → Y) (set : X → Y' → X')
     : Prop := WRITE {
     write {q t d xπ v} :
-      q.[α] -∗ ⟦ T.1 t d xπ [v] ⟧ᶜ =[rust_halt_wsat]{⊤}=∗ ∃ l wl du,
+      q.[κ] -∗ ⟦ T.1 t d xπ [v] ⟧ᶜ =[rust_halt_wsat]{⊤}=∗ ∃ l wl du,
         ⌜v = # l⌝ ∗ l ↦∗ wl ∗ ⟦ U.1 t du (get ∘ xπ) wl ⟧ᶜ ∗
         (∀ du' yπ' wl', l ↦∗ wl' -∗ ⟦ U'.1 t du' yπ' wl' ⟧ᶜ
           =[rust_halt_wsat]{⊤}=∗ ∃ d',
-          q.[α] ∗ ⟦ T'.1 t d' (λ π, set (xπ π) (yπ' π)) [v] ⟧ᶜ);
+          q.[κ] ∗ ⟦ T'.1 t d' (λ π, set (xπ π) (yπ' π)) [v] ⟧ᶜ);
   }.
 
   (** Reading a value from a pointer *)
   Lemma type_read v
     `(!EtcxExtract (X:=X) (Yl:=Zl) (Zl:=Zl') (v ◁ T) Γ Γr get' getr,
-      !Read (Y:=Y) (X':=X') α T U T' get set, !Ty U 1) :
-    ⊢ type α Γ (!v) (λ r, r ◁ U ᵖ:: v ◁ T' ᵖ:: Γr)
+      !Read (Y:=Y) (X':=X') κ T U T' get set, !Ty U 1) :
+    ⊢ type κ Γ (!v) (λ r, r ◁ U ᵖ:: v ◁ T' ᵖ:: Γr)
       (λ post zl, let x := get' zl in post (get x, set x, getr zl)').
   Proof.
-    rewrite type_unseal. iIntros (????) "!> α t pre".
+    rewrite type_unseal. iIntros (????) "!> κ t pre".
     rewrite etcx_extract /=. iIntros "[[% T] Γr]".
-    iMod (read with "α t T") as (? wl ?? ->) "(↦ & U & →T')".
+    iMod (read with "κ t T") as (? wl ?? ->) "(↦ & U & →T')".
     iDestruct (ty_own_size with "U") as %?. destruct wl as [|w[|??]]=>//.
     rewrite heap_pointsto_vec_singleton. wp_read.
     iMod ("→T'" with "↦") as (?) "($ & $ & T')". iModIntro. iFrame "pre".
@@ -84,13 +84,13 @@ Section read_write.
   (** Writing a value to a pointer *)
   Lemma type_write v w
     `(!TcxExtract (Xl:=[X;Y]) (Yl:=Zl) (Zl:=Zl') ᵖ[v ◁ T; w ◁ U] Γ Γr get' getr,
-      !Write (Y:=Y') (X':=X') α T U' U T' get set, !Ty U' 1) :
-    ⊢ type α Γ (v <- w) (λ _, v ◁ T' ᵖ:: Γr)
+      !Write (Y:=Y') (X':=X') κ T U' U T' get set, !Ty U' 1) :
+    ⊢ type κ Γ (v <- w) (λ _, v ◁ T' ᵖ:: Γr)
         (λ post zl, let '(x, y, _)' := get' zl in post (set x y, getr zl)').
   Proof.
-    rewrite type_unseal. iIntros (????) "!> α $ pre". rewrite tcx_extract /=.
+    rewrite type_unseal. iIntros (????) "!> κ $ pre". rewrite tcx_extract /=.
     iIntros "[([% T] & [% U] & _) Γr]".
-    iMod (write with "α T") as (? wl ? ->) "(↦ & U' & →T')".
+    iMod (write with "κ T") as (? wl ? ->) "(↦ & U' & →T')".
     iDestruct (ty_own_size with "U'") as %?. destruct wl as [|?[|??]]=>//.
     rewrite heap_pointsto_vec_singleton. wp_write.
     rewrite -heap_pointsto_vec_singleton.
@@ -101,16 +101,16 @@ Section read_write.
   Lemma type_memcopy vs vt
     `(!TcxExtract (Xl:=[Xs; Xt]) (Yl:=Zl) (Zl:=Zl') ᵖ[vs ◁ Ts; vt ◁ Tt] Γ Γr
         get getr,
-      !Read (Y:=Y) (X':=Xs') α Ts U Ts' gets sets,
-      !Write (Y:=Y') (X':=Xt') α Tt U' U Tt' gett sett, !Ty U sz, !Ty U' sz) :
-    ⊢ type α Γ (vt <-{sz} !vs)%E (λ _, vs ◁ Ts' ᵖ:: vt ◁ Tt' ᵖ:: Γr)
+      !Read (Y:=Y) (X':=Xs') κ Ts U Ts' gets sets,
+      !Write (Y:=Y') (X':=Xt') κ Tt U' U Tt' gett sett, !Ty U sz, !Ty U' sz) :
+    ⊢ type κ Γ (vt <-{sz} !vs)%E (λ _, vs ◁ Ts' ᵖ:: vt ◁ Tt' ᵖ:: Γr)
         (λ post zl, let '(xs, xt, _)' := get zl in
           post (sets xs, sett xt (gets xs), getr zl)').
   Proof.
-    rewrite type_unseal. iIntros (????) "!> [α α'] t pre".
+    rewrite type_unseal. iIntros (????) "!> [κ κ'] t pre".
     rewrite tcx_extract /=. iIntros "[([% Ts] & [% Tt] & _) Γr]".
-    iMod (read with "α t Ts") as (? wls ?? ->) "(↦s & U & →Ts')".
-    iMod (write with "α' Tt") as (? wlt ? ->) "(↦t & U' & →Tt')".
+    iMod (read with "κ t Ts") as (? wls ?? ->) "(↦s & U & →Ts')".
+    iMod (write with "κ' Tt") as (? wlt ? ->) "(↦t & U' & →Tt')".
     iDestruct (ty_own_size with "U") as %?.
     iDestruct (ty_own_size with "U'") as %?.
     wp_apply (twp_memcpy wls wlt with "[$↦s $↦t]")=>//. iIntros "[↦s ↦t]".
