nola/examples/rust_halt/core.v
@@ -12,15 +12,15 @@ Section type.
 
   (** Leak *)
   Lemma sub_leak {Xl} Γ
-    `(!TcxExtract (Xl:=Xl) (Yl:=Yl) (Zl:=Zl) Γ Γg Γr get getr) {α} :
-    ⊢ sub α Γg Γr (λ post yl, post (getr yl)).
+    `(!TcxExtract (Xl:=Xl) (Yl:=Yl) (Zl:=Zl) Γ Γg Γr get getr) {κ} :
+    ⊢ sub κ Γg Γr (λ post yl, post (getr yl)).
   Proof.
     rewrite sub_unseal. iIntros (????) "!>/= $ $ ?". rewrite tcx_extract.
     by iIntros "[_ $]".
   Qed.
   Lemma sub_leak_rest {Xl} Γ
-    `(!TcxExtract (Xl:=Xl) (Yl:=Yl) (Zl:=Zl) Γ Γg Γr get getr) {α} :
-    ⊢ sub α Γg Γ (λ post yl, post (get yl)).
+    `(!TcxExtract (Xl:=Xl) (Yl:=Yl) (Zl:=Zl) Γ Γg Γr get getr) {κ} :
+    ⊢ sub κ Γg Γ (λ post yl, post (get yl)).
   Proof.
     rewrite sub_unseal. iIntros (????) "!>/= $ $ ?". rewrite tcx_extract.
     by iIntros "[$ _]".
@@ -28,9 +28,9 @@ Section type.
   (** Modify by subtyping *)
   Lemma sub_subty v {X} T
     `(!EtcxExtract (X:=X) (Yl:=Zl) (Zl:=Zl') (v ◁ T) Γ Γr get getr)
-    {Y} U (f : X → Y) {α} :
+    {Y} U (f : X → Y) {κ} :
     subtyd T U f ⊢
-      sub α Γ (v ◁ U ᵖ:: Γr) (λ post zl, post (f (get zl), getr zl)').
+      sub κ Γ (v ◁ U ᵖ:: Γr) (λ post zl, post (f (get zl), getr zl)').
   Proof.
     rewrite subty_unseal sub_unseal. iIntros "[#TU _] !>/=" (????) "$ $ pre".
     rewrite etcx_extract. iIntros "[[% T] Γr] !>". iFrame "pre Γr".
@@ -38,9 +38,9 @@ Section type.
   Qed.
   Lemma sub_subty_frozen v {X} T
     `(!EtcxExtract (X:=X) (Yl:=Zl) (Zl:=Zl') (v ◁[†α] T) Γ Γr get getr)
-    {Y} U f `(!@Inj X Y (=) (=) f) {β} :
+    {Y} U f `(!@Inj X Y (=) (=) f) {κ} :
     subtyd T U f ⊢
-      sub β Γ (v ◁[†α] U ᵖ:: Γr) (λ post zl, post (f (get zl), getr zl)').
+      sub κ Γ (v ◁[†α] U ᵖ:: Γr) (λ post zl, post (f (get zl), getr zl)').
   Proof.
     rewrite subty_unseal sub_unseal. iIntros "[#TU _] !>/=" (????) "$ $ pre".
     rewrite etcx_extract. iIntros "[→T Γr] !>". iFrame "pre Γr". iIntros "†".
@@ -51,31 +51,31 @@ Section type.
   (** ** Basic typing rules *)
 
   (** Pure execution *)
-  Lemma type_pure {Xl Yl α Γi e e' Γo pre n φ} :
+  Lemma type_pure {Xl Yl κ Γi e e' Γo pre n φ} :
     PureExec φ n e e' → φ →
-    type (Xl:=Xl) (Yl:=Yl) α Γi e' Γo pre ⊢ type α Γi e Γo pre.
+    type (Xl:=Xl) (Yl:=Yl) κ Γi e' Γo pre ⊢ type κ Γi e Γo pre.
   Proof.
-    rewrite type_unseal=> ??. iIntros "#type !>" (????) "α t pre Γ".
-    wp_pure _. iApply ("type" with "α t pre Γ").
+    rewrite type_unseal=> ??. iIntros "#type !>" (????) "κ t pre Γ".
+    wp_pure _. iApply ("type" with "κ t pre Γ").
   Qed.
 
   (** Binding *)
-  Lemma type_bind {Xl Yl Zl α Γ Γ' Γ'' pre pre'} K e :
-    type (Yl:=Yl) α Γ e Γ' pre -∗
-    (∀ v, type α (Γ' v) (fill K (of_val v)) Γ'' pre') -∗
-      type (Xl:=Xl) (Yl:=Zl) α Γ (fill K e) Γ'' (pre ∘ pre').
+  Lemma type_bind {Xl Yl Zl κ Γ Γ' Γ'' pre pre'} K e :
+    type (Yl:=Yl) κ Γ e Γ' pre -∗
+    (∀ v, type κ (Γ' v) (fill K (of_val v)) Γ'' pre') -∗
+      type (Xl:=Xl) (Yl:=Zl) κ Γ (fill K e) Γ'' (pre ∘ pre').
   Proof.
-    rewrite type_unseal. iIntros "#type #type' !>" (????) "α t pre Γ".
-    iApply twp_bind. iDestruct ("type" with "α t pre Γ") as "big".
-    iApply (twp_wand with "big"). iIntros (?) ">(% & α & t & pre & Γ')".
-    iApply ("type'" with "α t pre Γ'").
+    rewrite type_unseal. iIntros "#type #type' !>" (????) "κ t pre Γ".
+    iApply twp_bind. iDestruct ("type" with "κ t pre Γ") as "big".
+    iApply (twp_wand with "big"). iIntros (?) ">(% & κ & t & pre & Γ')".
+    iApply ("type'" with "κ t pre Γ'").
   Qed.
   (** Let expression *)
-  Lemma type_let {Xl Yl Zl α Γ Γ' Γ'' x e e' pre pre'}
+  Lemma type_let {Xl Yl Zl κ Γ Γ' Γ'' x e e' pre pre'}
     `{!Closed (x :b: []) e'} :
-    type (Yl:=Yl) α Γ e Γ' pre -∗
-    (∀ v, type α (Γ' v) (subst' x v e') Γ'' pre') -∗
-      type (Xl:=Xl) (Yl:=Zl) α Γ (let: x := e in e') Γ'' (pre ∘ pre').
+    type (Yl:=Yl) κ Γ e Γ' pre -∗
+    (∀ v, type κ (Γ' v) (subst' x v e') Γ'' pre') -∗
+      type (Xl:=Xl) (Yl:=Zl) κ Γ (let: x := e in e') Γ'' (pre ∘ pre').
   Proof.
     iIntros "#type #type'". iApply (type_bind [LetCtx x e'] with "type")=>/=.
     iIntros (?). by iApply (type_pure with "type'").
@@ -84,64 +84,64 @@ Section type.
   (** ** Operations on lifetimes *)
 
   (** Allocate a new local lifetime *)
-  Lemma type_lft_new {Xl Yl β Γi e Γo pre} :
-    (∀ α, type β (^[α] ᵖ:: Γi) e Γo pre) ⊢
-      type (Xl:=Xl) (Yl:=Yl) β Γi e Γo (λ post xl, pre post ((), xl)').
+  Lemma type_lft_new {Xl Yl κ Γi e Γo pre} :
+    (∀ α, type κ (^[α] ᵖ:: Γi) e Γo pre) ⊢
+      type (Xl:=Xl) (Yl:=Yl) κ Γi e Γo (λ post xl, pre post ((), xl)').
   Proof.
     rewrite type_unseal.
-    iIntros "#type !>" (????) "β t pre Γi". iMod lft_alloc as (α ?) "α".
-    iApply ("type" with "β t pre"). by iFrame.
+    iIntros "#type !>" (????) "κ t pre Γi". iMod lft_alloc as (α ?) "α".
+    iApply ("type" with "κ t pre"). by iFrame.
   Qed.
   (** Use a local lifetime *)
   Lemma type_lft_use α
-    `(!EtcxExtract (Yl:=Xl) (Zl:=Xl') ^[α] Γi Γr get getr) {Yl β e Γo pre} :
-    type (Yl:=Yl) (α ⊓ β) Γr e Γo pre ⊢
-      type β Γi e (λ v, ^[α] ᵖ:: Γo v)
+    `(!EtcxExtract (Yl:=Xl) (Zl:=Xl') ^[α] Γi Γr get getr) {Yl κ e Γo pre} :
+    type (Yl:=Yl) (α ⊓ κ) Γr e Γo pre ⊢
+      type κ Γi e (λ v, ^[α] ᵖ:: Γo v)
         (λ post xl, pre (λ yl, post ((), yl)') (getr xl)).
   Proof.
-    rewrite type_unseal. iIntros "#type !>/=" (q ???) "β t pre Γi".
+    rewrite type_unseal. iIntros "#type !>/=" (q ???) "κ t pre Γi".
     rewrite etcx_extract. iDestruct "Γi" as "[[% α] Γr]".
     case (Qp.lower_bound 1 q) as [?[?[?[->->]]]]. iDestruct "α" as "[α $]".
-    iDestruct "β" as "[β $]".
-    iDestruct ("type" with "[$α $β //] t pre Γr") as "twp".
+    iDestruct "κ" as "[κ $]".
+    iDestruct ("type" with "[$α $κ //] t pre Γr") as "twp".
     iApply (twp_wand with "twp"). by iIntros (?) ">(% & [$$] & $ & $ & $) !>".
   Qed.
   (** Eternalize a lifetime *)
   Lemma sub_lft_eternal α
-    `(!EtcxExtract (Yl:=Xl) (Zl:=Xl') ^[α] Γi Γr get getr) {Yl β Γo pre} :
-    □ ((∀ α', α' ⊑□ α) -∗ sub (Yl:=Yl) β Γr Γo pre) ⊢
-      sub β Γi Γo (λ post xl, pre post (getr xl)).
+    `(!EtcxExtract (Yl:=Xl) (Zl:=Xl') ^[α] Γi Γr get getr) {Yl κ Γo pre} :
+    □ ((∀ β, β ⊑□ α) -∗ sub (Yl:=Yl) κ Γr Γo pre) ⊢
+      sub κ Γi Γo (λ post xl, pre post (getr xl)).
   Proof.
-    rewrite sub_unseal. iIntros "#sub !>/=" (????) "β t pre Γi".
+    rewrite sub_unseal. iIntros "#sub !>/=" (????) "κ t pre Γi".
     rewrite etcx_extract. iDestruct "Γi" as "[[% α] Γr]".
     iMod (lft_eternalize_sincl with "α") as "∞"=>//.
-    iApply ("sub" with "∞ β t pre Γr").
+    iApply ("sub" with "∞ κ t pre Γr").
   Qed.
   Lemma type_lft_eternal α
     `(!EtcxExtract (Yl:=Xl) (Zl:=Xl') ^[α] Γi Γr get getr)
-    {Yl Zl β Γi' e Γo pre pre'} :
-    □ ((∀ α', α' ⊑□ α) -∗ sub (Yl:=Yl) β Γr Γi' pre) -∗
-    type (Yl:=Zl) β Γi' e Γo pre' -∗
-      type β Γi e Γo (λ post xl, pre (pre' post) (getr xl)).
+    {Yl Zl κ Γi' e Γo pre pre'} :
+    □ ((∀ β, β ⊑□ α) -∗ sub (Yl:=Yl) κ Γr Γi' pre) -∗
+    type (Yl:=Zl) κ Γi' e Γo pre' -∗
+      type κ Γi e Γo (λ post xl, pre (pre' post) (getr xl)).
   Proof.
     iIntros "#sub #type". iApply type_pre; last first.
     { iApply type_in; [|done]. by iApply sub_lft_eternal. } { done. }
   Qed.
   (** End a lifetime *)
   Lemma sub_lft_end α
-    `(!EtcxExtract (Yl:=Xl) (Zl:=Xl') ^[α] Γi Γr get getr) {Yl β Γo pre} :
-    □ ([†α] -∗ sub (Yl:=Yl) β Γr Γo pre) ⊢
-      sub β Γi Γo (λ post xl, pre post (getr xl)).
+    `(!EtcxExtract (Yl:=Xl) (Zl:=Xl') ^[α] Γi Γr get getr) {Yl κ Γo pre} :
+    □ ([†α] -∗ sub (Yl:=Yl) κ Γr Γo pre) ⊢
+      sub κ Γi Γo (λ post xl, pre post (getr xl)).
   Proof.
-    rewrite sub_unseal. iIntros "#sub !>/=" (????) "β t pre Γi".
+    rewrite sub_unseal. iIntros "#sub !>/=" (????) "κ t pre Γi".
     rewrite etcx_extract. iDestruct "Γi" as "[[% α] Γr]".
-    iMod (lft_kill with "α") as "†"=>//. iApply ("sub" with "† β t pre Γr").
+    iMod (lft_kill with "α") as "†"=>//. iApply ("sub" with "† κ t pre Γr").
   Qed.
   Lemma type_lft_end α
     `(!EtcxExtract (Yl:=Xl) (Zl:=Xl') ^[α] Γi Γr get getr)
-    {Yl Zl β Γi' e Γo pre pre'} :
-    □ ([†α] -∗ sub (Yl:=Yl) β Γr Γi' pre) -∗ type (Yl:=Zl) β Γi' e Γo pre' -∗
-      type β Γi e Γo (λ post xl, pre (pre' post) (getr xl)).
+    {Yl Zl κ Γi' e Γo pre pre'} :
+    □ ([†α] -∗ sub (Yl:=Yl) κ Γr Γi' pre) -∗ type (Yl:=Zl) κ Γi' e Γo pre' -∗
+      type κ Γi e Γo (λ post xl, pre (pre' post) (getr xl)).
   Proof.
     iIntros "#sub #type". iApply type_pre; last first.
     { iApply type_in; [|done]. by iApply sub_lft_end. } { done. }
@@ -149,13 +149,13 @@ Section type.
   (** Retrieve a frozen object *)
   Lemma sub_retrieve v α
     `(!EtcxExtract (X:=X) (Yl:=Yl) (Zl:=Zl) (v ◁[†α] T) Γ Γr get getr,
-      !TyOp T β) :
-    [†α] -∗ sub β Γ (v ◁ T ᵖ:: Γr) (λ post yl, post (get yl, getr yl)').
+      !TyOp T κ) :
+    [†α] -∗ sub κ Γ (v ◁ T ᵖ:: Γr) (λ post yl, post (get yl, getr yl)').
   Proof.
-    rewrite sub_unseal. iIntros "#† !>/=" (????) "β $ pre".
+    rewrite sub_unseal. iIntros "#† !>/=" (????) "κ $ pre".
     rewrite etcx_extract /=. iIntros "[→T Γr]".
     iMod ("→T" with "†") as (? xπ') "[eqz T]".
-    iMod (ty_own_proph with "β T") as (???) "[ξl cl]".
+    iMod (ty_own_proph with "κ T") as (???) "[ξl cl]".
     iMod ("eqz" with "[//] ξl") as "[ξl eq]". iMod ("cl" with "ξl") as "[$ T]".
     iModIntro. iExists (λ π, (xπ' π, _)')=>/=. iFrame "T Γr".
     by iApply (proph_obs_impl2 with "pre eq")=> ??<-.
