nola/examples/rust_halt/num.v
@@ -35,15 +35,15 @@ Section num.
   Proof. iApply (subty_pty pty_bool pty_nat). by iIntros ([|]?). Qed.
 
   (** Integer operations *)
-  Lemma type_int (n : Z) {α Xl Γ} :
-    ⊢ type (Xl:=Xl) α Γ #n (λ r, r ◁ ty_int ᵖ:: Γ) (λ post xl, post (n, xl)').
+  Lemma type_int (n : Z) {κ Xl Γ} :
+    ⊢ type (Xl:=Xl) κ Γ #n (λ r, r ◁ ty_int ᵖ:: Γ) (λ post xl, post (n, xl)').
   Proof.
     rewrite /= type_unseal. iIntros (????) "!>/= $ $ pre Γ". wp_value_head.
     iModIntro. iFrame "pre Γ". iPureIntro. eexists 0, _. split=>//=.
   Qed.
-  Lemma type_add_int v v' {α}
+  Lemma type_add_int v v' {κ}
     `(!TcxExtract (Yl:=Xl) (Zl:=Yl) ᵖ[v ◁ ty_int; v' ◁ ty_int] Γi Γr get getr) :
-    ⊢ type α Γi (v + v') (λ r, r ◁ ty_int ᵖ:: Γr)
+    ⊢ type κ Γi (v + v') (λ r, r ◁ ty_int ᵖ:: Γr)
       (λ post xl, let '(n, n', _)' := get xl in post (n + n', getr xl)'%Z).
   Proof.
     rewrite /= type_unseal. iIntros (????) "!>/= $ $ pre". rewrite tcx_extract.
@@ -52,9 +52,9 @@ Section num.
     iModIntro. iFrame "pre Γr". iPureIntro. eexists 0, _. split=>//= ?.
     by rewrite eq eq'.
   Qed.
-  Lemma type_sub_int v v' {α}
+  Lemma type_sub_int v v' {κ}
     `(!TcxExtract (Yl:=Xl) (Zl:=Yl) ᵖ[v ◁ ty_int; v' ◁ ty_int] Γi Γr get getr) :
-    ⊢ type α Γi (v - v') (λ r, r ◁ ty_int ᵖ:: Γr)
+    ⊢ type κ Γi (v - v') (λ r, r ◁ ty_int ᵖ:: Γr)
       (λ post xl, let '(n, n', _)' := get xl in post (n - n', getr xl)'%Z).
   Proof.
     rewrite /= type_unseal. iIntros (????) "!>/= $ $ pre". rewrite tcx_extract.
@@ -63,9 +63,9 @@ Section num.
     iModIntro. iFrame "pre Γr". iPureIntro. eexists 0, _. split=>//= ?.
     by rewrite eq eq'.
   Qed.
-  Lemma type_eq_int v v' {α}
+  Lemma type_eq_int v v' {κ}
     `(!TcxExtract (Yl:=Xl) (Zl:=Yl) ᵖ[v ◁ ty_int; v' ◁ ty_int] Γi Γr get getr) :
-    ⊢ type α Γi (v = v') (λ r, r ◁ ty_bool ᵖ:: Γr)
+    ⊢ type κ Γi (v = v') (λ r, r ◁ ty_bool ᵖ:: Γr)
       (λ post xl, let '(n, n', _)' := get xl in
         post (bool_decide (n = n'), getr xl)').
   Proof.
@@ -75,9 +75,9 @@ Section num.
     iModIntro. iFrame "pre Γr". iPureIntro. eexists 0, _. split=>//= ?.
     by rewrite eq eq'.
   Qed.
-  Lemma type_le_int v v' {α}
+  Lemma type_le_int v v' {κ}
     `(!TcxExtract (Yl:=Xl) (Zl:=Yl) ᵖ[v ◁ ty_int; v' ◁ ty_int] Γi Γr get getr) :
-    ⊢ type α Γi (v ≤ v') (λ r, r ◁ ty_bool ᵖ:: Γr)
+    ⊢ type κ Γi (v ≤ v') (λ r, r ◁ ty_bool ᵖ:: Γr)
       (λ post xl, let '(n, n', _)' := get xl in
         post (bool_decide (n ≤ n')%Z, getr xl)').
   Proof.
@@ -89,15 +89,15 @@ Section num.
   Qed.
 
   (** Natural number operations *)
-  Lemma type_nat (n : nat) {α Xl Γ} :
-    ⊢ type (Xl:=Xl) α Γ #n (λ r, r ◁ ty_nat ᵖ:: Γ) (λ post xl, post (n, xl)').
+  Lemma type_nat (n : nat) {κ Xl Γ} :
+    ⊢ type (Xl:=Xl) κ Γ #n (λ r, r ◁ ty_nat ᵖ:: Γ) (λ post xl, post (n, xl)').
   Proof.
     rewrite /= type_unseal. iIntros (????) "!>/= $ $ pre Γ". wp_value_head.
     iModIntro. iFrame "pre Γ". iPureIntro. eexists 0, _. split=>//=.
   Qed.
-  Lemma type_add_nat v v' {α}
+  Lemma type_add_nat v v' {κ}
     `(!TcxExtract (Yl:=Xl) (Zl:=Yl) ᵖ[v ◁ ty_nat; v' ◁ ty_nat] Γi Γr get getr) :
-    ⊢ type α Γi (v + v') (λ r, r ◁ ty_nat ᵖ:: Γr)
+    ⊢ type κ Γi (v + v') (λ r, r ◁ ty_nat ᵖ:: Γr)
       (λ post xl, let '(n, n', _)' := get xl in post (n + n', getr xl)').
   Proof.
     rewrite /= type_unseal. iIntros (????) "!>/= $ $ pre". rewrite tcx_extract.
@@ -106,9 +106,9 @@ Section num.
     iModIntro. iFrame "pre Γr". iPureIntro. eexists 0, _. split=>/=.
     { move=> ?. by rewrite eq eq'. } { do 3 f_equal. lia. }
   Qed.
-  Lemma type_sub_nat v v' {α}
+  Lemma type_sub_nat v v' {κ}
     `(!TcxExtract (Yl:=Xl) (Zl:=Yl) ᵖ[v ◁ ty_nat; v' ◁ ty_nat] Γi Γr get getr) :
-    ⊢ type α Γi (v - v') (λ r, r ◁ ty_nat ᵖ:: Γr)
+    ⊢ type κ Γi (v - v') (λ r, r ◁ ty_nat ᵖ:: Γr)
       (λ post xl, let '(n, n', _)' := get xl in
         n ≥ n' ∧ post (n - n', getr xl)')%type.
   Proof.
@@ -122,9 +122,9 @@ Section num.
     rewrite proph_obs_sat. iRevert "pre". iPureIntro. case=>/= [?+].
     rewrite eq eq'. case=> ??. do 3 f_equal. lia.
   Qed.
-  Lemma type_eq_nat v v' {α}
+  Lemma type_eq_nat v v' {κ}
     `(!TcxExtract (Yl:=Xl) (Zl:=Yl) ᵖ[v ◁ ty_nat; v' ◁ ty_nat] Γi Γr get getr) :
-    ⊢ type α Γi (v = v') (λ r, r ◁ ty_bool ᵖ:: Γr)
+    ⊢ type κ Γi (v = v') (λ r, r ◁ ty_bool ᵖ:: Γr)
       (λ post xl, let '(n, n', _)' := get xl in
         post (bool_decide (n = n'), getr xl)').
   Proof.
@@ -134,9 +134,9 @@ Section num.
     iModIntro. iFrame "pre Γr". iPureIntro. eexists 0, _. split=>//= ?.
     rewrite eq eq'. apply bool_decide_ext. lia.
   Qed.
-  Lemma type_le_nat v v' {α}
+  Lemma type_le_nat v v' {κ}
     `(!TcxExtract (Yl:=Xl) (Zl:=Yl) ᵖ[v ◁ ty_nat; v' ◁ ty_nat] Γi Γr get getr) :
-    ⊢ type α Γi (v ≤ v') (λ r, r ◁ ty_bool ᵖ:: Γr)
+    ⊢ type κ Γi (v ≤ v') (λ r, r ◁ ty_bool ᵖ:: Γr)
       (λ post xl, let '(n, n', _)' := get xl in
         post (bool_decide (n ≤ n'), getr xl)').
   Proof.
@@ -146,8 +146,8 @@ Section num.
     iModIntro. iFrame "pre Γr". iPureIntro. eexists 0, _. split=>//= ?.
     rewrite eq eq'. apply bool_decide_ext. lia.
   Qed.
-  Lemma type_ndnat {α Xl Γ} :
-    ⊢ type (Xl:=Xl) α Γ Ndnat (λ r, r ◁ ty_nat ᵖ:: Γ)
+  Lemma type_ndnat {κ Xl Γ} :
+    ⊢ type (Xl:=Xl) κ Γ Ndnat (λ r, r ◁ ty_nat ᵖ:: Γ)
       (λ post xl, ∀ n, post (n ᵖ:: xl))%type.
   Proof.
     rewrite /= type_unseal. iIntros (????) "!>/= $ $ pre Γ".
@@ -157,16 +157,16 @@ Section num.
   Qed.
 
   (** Boolean operations *)
-  Lemma type_bool (b : bool) {α Xl Γ} :
-    ⊢ type (Xl:=Xl) α Γ #b (λ r, r ◁ ty_bool ᵖ:: Γ) (λ post xl, post (b, xl)').
+  Lemma type_bool (b : bool) {κ Xl Γ} :
+    ⊢ type (Xl:=Xl) κ Γ #b (λ r, r ◁ ty_bool ᵖ:: Γ) (λ post xl, post (b, xl)').
   Proof.
     rewrite /= type_unseal. iIntros (????) "!>/= $ $ pre Γ". wp_value_head.
     iModIntro. iFrame "pre Γ". iPureIntro. eexists 0, _. split=>//=.
   Qed.
-  Lemma type_eq_bool v v' {α}
+  Lemma type_eq_bool v v' {κ}
     `(!TcxExtract (Yl:=Xl) (Zl:=Yl) ᵖ[v ◁ ty_bool; v' ◁ ty_bool]
         Γi Γr get getr) :
-    ⊢ type α Γi (v = v') (λ r, r ◁ ty_bool ᵖ:: Γr)
+    ⊢ type κ Γi (v = v') (λ r, r ◁ ty_bool ᵖ:: Γr)
       (λ post xl, let '(b, b', _)' := get xl in
         post (bool_decide (b = b'), getr xl)').
   Proof.
@@ -176,10 +176,10 @@ Section num.
     iModIntro. iFrame "pre Γr". iPureIntro. eexists 0, _. split=>//= ?.
     rewrite eq eq'. apply bool_decide_ext. by case b; case b'.
   Qed.
-  Lemma type_le_bool v v' {α}
+  Lemma type_le_bool v v' {κ}
     `(!TcxExtract (Yl:=Xl) (Zl:=Yl) ᵖ[v ◁ ty_bool; v' ◁ ty_bool]
         Γi Γr get getr) :
-    ⊢ type α Γi (v ≤ v') (λ r, r ◁ ty_bool ᵖ:: Γr)
+    ⊢ type κ Γi (v ≤ v') (λ r, r ◁ ty_bool ᵖ:: Γr)
       (λ post xl, let '(b, b', _)' := get xl in
         post (negb b || b', getr xl)').
   Proof.
@@ -193,16 +193,16 @@ Section num.
   (** If expression *)
   Lemma type_if v
     `(!EtcxExtract (Yl:=Xl) (Zl:=Yl) (v ◁ ty_bool) Γi Γr get getr)
-    {Zl α e e' Γo pre pre'} :
-    type (Yl:=Zl) α Γr e Γo pre -∗ type α Γr e' Γo pre' -∗
-      type α Γi (if: v then e else e') Γo
+    {Zl κ e e' Γo pre pre'} :
+    type (Yl:=Zl) κ Γr e Γo pre -∗ type κ Γr e' Γo pre' -∗
+      type κ Γi (if: v then e else e') Γo
         (λ post xl, if get xl then pre post (getr xl) else pre' post (getr xl)).
   Proof.
-    rewrite /= type_unseal. iIntros "#type #type' !>/=" (????) "α t #pre".
+    rewrite /= type_unseal. iIntros "#type #type' !>/=" (????) "κ t #pre".
     rewrite etcx_extract. iIntros "/=[%vb Γr]".
     destruct vb as (? & b & eq & [= ->]).
     destruct b; wp_if;
-      [iApply ("type" with "α t [] Γr")|iApply ("type'" with "α t [] Γr")];
+      [iApply ("type" with "κ t [] Γr")|iApply ("type'" with "κ t [] Γr")];
       iApply (proph_obs_impl with "pre")=> ?; by rewrite eq.
   Qed.
 
@@ -220,29 +220,29 @@ Section num.
         S n' => pre (λ '(x', zl')', pre_nat_iter n' x' zl') (n', x, zl)' end.
   End pre_nat_iter.
   (** Typing [nat_iter] *)
-  Lemma type'_nat_iter {f : val} {α X T Zl v w Γ pre} :
-    (∀ v w, type (Xl:=_::X::Zl) α (v ◁ ty_nat ᵖ:: w ◁ T ᵖ:: Γ) (f [v; w]%E)
+  Lemma type'_nat_iter {f : val} {κ X T Zl v w Γ pre} :
+    (∀ v w, type (Xl:=_::X::Zl) κ (v ◁ ty_nat ᵖ:: w ◁ T ᵖ:: Γ) (f [v; w]%E)
       (λ r, r ◁ T ᵖ:: Γ) pre) ⊢
-    type α (v ◁ ty_nat ᵖ:: w ◁ T ᵖ:: Γ) (nat_iter [f; v; w]%E)
+    type κ (v ◁ ty_nat ᵖ:: w ◁ T ᵖ:: Γ) (nat_iter [f; v; w]%E)
       (λ r, r ◁ T ᵖ:: Γ) (λ post '(n, x, zl)', pre_nat_iter pre post n x zl).
   Proof.
     rewrite /= type_unseal.
-    iIntros "#type !>/=" (?? postπ xlπ) "α t pre (%vi & [%d T] & Γ)".
+    iIntros "#type !>/=" (?? postπ xlπ) "κ t pre (%vi & [%d T] & Γ)".
     destruct vi as (? & n & eq & [= ->]). setoid_rewrite eq. clear.
     iInduction n as [|n'] "IH" forall (postπ xlπ d w); wp_rec; wp_op; wp_case.
     { iModIntro. do 2 iFrame. }
     wp_op. have -> : (S n' - 1)%Z = n' by lia. wp_let. wp_bind (f _).
-    iDestruct ("type" with "α t pre [T Γ]") as "twp"=>/=.
+    iDestruct ("type" with "κ t pre [T Γ]") as "twp"=>/=.
     { iFrame. by iExists 0, _. }
-    iApply (twp_wand with "twp"). iIntros (?) ">(% & α & t & pre & [% T] & Γ)".
-    iApply ("IH" $! _ (λ _,(0,_)') with "α t pre T Γ").
+    iApply (twp_wand with "twp"). iIntros (?) ">(% & κ & t & pre & [% T] & Γ)".
+    iApply ("IH" $! _ (λ _,(0,_)') with "κ t pre T Γ").
   Qed.
-  Lemma type_nat_iter {α X T} {f : val}
+  Lemma type_nat_iter {κ X T} {f : val}
     `(!TcxExtract (Xl:=[_;X]) (Yl:=Yl) (Zl:=Zl) ᵖ[v ◁ ty_nat; w ◁ T] Γi Γr
         get getr) {pre} :
-    (∀ v w, type α (v ◁ ty_nat ᵖ:: w ◁ T ᵖ:: Γr) (f [v; w]%E)
+    (∀ v w, type κ (v ◁ ty_nat ᵖ:: w ◁ T ᵖ:: Γr) (f [v; w]%E)
       (λ r, r ◁ T ᵖ:: Γr) pre) ⊢
-    type α Γi (nat_iter [f; v; w]%E) (λ r, r ◁ T ᵖ:: Γr)
+    type κ Γi (nat_iter [f; v; w]%E) (λ r, r ◁ T ᵖ:: Γr)
       (λ post yl, let '(n, x, _)' := get yl in
         pre_nat_iter pre post n x (getr yl))%type.
   Proof.
